[rp] new rewriter feature 'equals' is added. With proved invariance, now meta functions (maybe rw rules in the future) can introduce terms of the form (equals term1 term2) where evalutation term1 and term2 are guaranteed to be the same. This can enable undoing a rewriting at some later time in case of a misstep.

books/projects/rp-rewriter/aux-functions.lisp
@@ -51,6 +51,10 @@
   (declare (ignorable prop))
   term)
 
+(defun equals (term1 term2)
+  (declare (ignorable term1 term2))
+  term1)
+
 (defun falist (fast-list term)
   (declare (ignorable fast-list))
   term)
@@ -135,6 +139,8 @@
        (cons (beta-search-reduce (car subterms) (1- limit))
              (beta-search-reduce-subterms (cdr subterms) (1- limit)))))))
 
+
+
 (define is-rp (term)
   :inline t
   (case-match term (('rp ('quote type) &)
@@ -155,6 +161,17 @@
                      (not (booleanp type))
                      (not (equal type 'quote))))
                (& nil)))))
+
+(define is-equals (term)
+  :inline t
+  (case-match term (('equals & &)
+                    t))
+  ///
+  (defthm is-equals-implies
+    (implies (is-equals term)
+             (case-match term (('equals & &) t)))
+    :rule-classes :forward-chaining))
+
 (define is-if (term)
   :inline t
   (case-match term (('if & & &) t)
@@ -539,29 +556,40 @@
          (not (quotep (car lst)))
          (cons-consp (cdr lst)))))
 
+
+
+(define maybe-natp (x)
+  :enabled t
+  (or (not x)
+      (natp x))) 
+
 (acl2::defines
  include-fnc
- (define include-fnc (term fnc)
+ (define include-fnc (term fnc &optional arg-size)
    :enabled t
-   :guard (symbolp fnc)
+   :guard (and (symbolp fnc)
+               (maybe-natp arg-size))
    :parents (rp-utilities)
    :short "Searches a term for an instance of fnc. Returns t or nil."
    (if (or (atom term)
            (quotep term))
        nil
-     (if (eq (car term) fnc)
+     (if (and (eq (car term) fnc)
+              (implies arg-size
+                       (equal (len (cdr term)) arg-size)))
          t
-       (include-fnc-subterms (cdr term) fnc))))
+       (include-fnc-subterms (cdr term) fnc arg-size))))
 
- (define include-fnc-subterms (subterms fnc)
-   :guard (symbolp fnc)
+ (define include-fnc-subterms (subterms fnc &optional arg-size)
+   :guard (and (symbolp fnc)
+               (maybe-natp arg-size))
    :enabled t
    :parents (include-fnc)
    :short "Searches a list of terms for an instance of fnc. Returns t or nil."
    (if (atom subterms)
        nil
-     (or (include-fnc (car subterms) fnc)
-         (include-fnc-subterms (cdr subterms) fnc)))))
+     (or (include-fnc (car subterms) fnc arg-size)
+         (include-fnc-subterms (cdr subterms) fnc arg-size)))))
 
 (defun is-honsed-assoc-eq-values (term)
   (declare (xargs :guard t))
@@ -1249,14 +1277,26 @@
             (and warning
                  (cw "ATTENTION! (not (include-fnc (rp-lhs rule) 'rp))
     failed! LHS cannot contain an instance of rp. ~%")))
+        (or (not (include-fnc (rp-lhs rule) 'equals))
+            (and warning
+                 (cw "ATTENTION! (not (include-fnc (rp-lhs rule) 'equals))
+    failed! LHS cannot contain an instance of equals. ~%")))
         (or (not (include-fnc-subterms (rp-hyp rule) 'rp))
             (and warning
                  (cw "ATTENTION! (not (include-fnc-subterms (rp-hyp rule) 'rp))
     failed! HYP cannot contain an instance of rp. ~%")))
+        (or (not (include-fnc-subterms (rp-hyp rule) 'equals))
+            (and warning
+                 (cw "ATTENTION! (not (include-fnc-subterms (rp-hyp rule) 'equals))
+    failed! HYP cannot contain an instance of equals ~%")))
         (or (not (include-fnc (rp-rhs rule) 'falist))
             (and warning
                  (cw "ATTENTION! (not (include-fnc (rp-rhs rule) 'falist))
     failed! RHS cannot contain an instance of falist ~%")))
+        (or (not (include-fnc (rp-rhs rule) 'equals))
+            (and warning
+                 (cw "ATTENTION! (not (include-fnc (rp-rhs rule) 'equals))
+    failed! RHS cannot contain an instance of equals ~%")))
         (or (not (include-fnc-subterms (rp-hyp rule) 'falist))
             (and warning
                  (cw "ATTENTION! (not (include-fnc (rp-hyp rule) 'falist))
@@ -1385,6 +1425,8 @@ In the hyps: ~p0, in the rhs :~p1. ~%")))|#
              (ex-from-rp-all2 (caddr term)))
             ((is-rp-loose term)
              (ex-from-rp-all2 (caddr term)))
+            ((is-equals term)
+             (ex-from-rp-all2 (cadr term)))
             (t
              (cons-with-hint (car term)
                              (ex-from-rp-all2-lst (cdr term))
