books/projects/rp-rewriter/lib/mult3/4vec-branch-drop-redundant-case.lisp
@@ -58,6 +58,13 @@
 (local
  (include-book "lemmas-2"))
 
+(local
+   (defthm is-equals-of-others
+     (implies (not (equal (car term) 'equals))
+              (not (is-equals term )))
+     :hints (("Goal"
+              :in-theory (e/d (is-equals) ())))))
+
 (define 4vec-branch-drop-r-case-pattern-check ((term rp-termp))
   :Returns (pass booleanp)
   :measure (cons-count term)
